ExistentialRules/ChaseSequence/Nontermination/RpcLike.lean
@@ -90,41 +90,71 @@ def derivation_for_skeleton
     apply cd.unblockable
     exact ChaseDerivationSkeleton.mem_of_mem_suffix suffix _ node_mem
 
-/-- We restate the `growing` property using vocabulary available for `ChaseDerivationSkeleton`s. -/
-theorem growing' {cd : CyclicityDerivation obs rules} : ∀ node : cd.Node,
+/-- We restate the `growing` property using suffix vocabulary available for `ChaseDerivationSkeleton`s. -/
+theorem growing' {cd : CyclicityDerivation obs rules} : ∃ cd2 : CyclicityDerivation obs rules, cd2.toChaseDerivationSkeleton <:+ cd.toChaseDerivationSkeleton ∧
+    ∃ t, t ∉ cd.head.facts.terms ∧ t ∈ cd2.head.facts.terms := by
+  rcases cd.growing 0 with ⟨m, t, t_not_mem, ⟨node, node_mem, t_mem⟩⟩
+  rw [Nat.zero_add] at node_mem
+  specialize t_not_mem cd.head (by simp [ChaseDerivationSkeleton.head])
+  let cd2 : ChaseDerivationSkeleton obs rules := cd.derivation_for_branch_suffix _ (cd.branch.IsSuffix_drop m) (by rw [node_mem]; simp)
+  have cd2_suffix : cd2 <:+ cd.toChaseDerivationSkeleton := cd.branch.IsSuffix_drop m
+  exists cd.derivation_for_skeleton cd2 cd2_suffix
+  constructor; exact cd2_suffix
+  exists t; constructor; exact t_not_mem
+  suffices cd2.head = node by simp only [derivation_for_skeleton, this]; exact t_mem
+  simp only [cd2, ChaseDerivationSkeleton.derivation_for_branch_suffix, ChaseDerivationSkeleton.head]
+  rw [Option.mem_def] at node_mem
+  simp [node_mem]
+
+/-- Given a list of terms, we can find a suffix that contains a term that is not part of this list because of the growing property. This result is closest to the `growing'` statement. -/
+theorem growing'_for_list (cd : CyclicityDerivation obs rules) (l : List (GroundTerm sig)) : ∃ cd2 : CyclicityDerivation obs rules,
+    cd2.toChaseDerivationSkeleton <:+ cd.toChaseDerivationSkeleton ∧ ∃ t, t ∉ cd.head.facts.terms ∧ t ∈ cd2.head.facts.terms ∧ t ∉ l := by
+  induction l generalizing cd with
+  | nil => rcases cd.growing' with ⟨cd2, suf, t, t_not_mem, t_mem⟩; exact ⟨cd2, suf, t, t_not_mem, t_mem, by simp⟩
+  | cons hd tl ih =>
+    rcases ih cd with ⟨cd2, suf, t, t_not_mem, t_mem, t_not_mem_l⟩
+    rcases ih cd2 with ⟨cd3, suf2, s, s_not_mem, s_mem, s_not_mem_l⟩
+    cases Decidable.em (hd = t) with
+    | inr ne => exists cd2; constructor; exact suf; exists t; grind
+    | inl eq =>
+      exists cd3; constructor; exact PossiblyInfiniteList.IsSuffix_trans suf2 suf
+      exists s
+      constructor
+      . intro contra; apply s_not_mem; apply FactSet.terms_subset_of_subset (cd.facts_node_subset_every_mem _ (ChaseDerivationSkeleton.mem_of_mem_suffix suf _ cd2.head_mem)); exact contra
+      constructor; exact s_mem
+      . intro contra; rw [List.mem_cons] at contra; cases contra with
+        | inr contra => apply s_not_mem_l; exact contra
+        | inl contra => apply s_not_mem; rw [contra, eq]; exact t_mem
+
+/-- We restate the `growing` property using predecessor vocabulary available for `ChaseDerivationSkeleton`s. -/
+theorem growing'' {cd : CyclicityDerivation obs rules} : ∀ node : cd.Node,
     ∃ node2 : cd.Node, node ≺ node2 ∧ ∃ t, ¬ t ∈ node.val.facts.terms ∧ t ∈ node2.val.facts.terms := by
   intro ⟨node, node_mem⟩
   rw [ChaseDerivationSkeleton.mem_iff] at node_mem
   rcases node_mem with ⟨n, node_eq⟩
-  rcases cd.growing n with ⟨m, t, t_not_mem, ⟨node2, node2_mem, t_mem⟩⟩
-  specialize t_not_mem node (by simpa using node_eq)
 
   let cd2 : ChaseDerivationSkeleton obs rules := cd.derivation_for_branch_suffix _ (cd.branch.IsSuffix_drop n) (by simp [node_eq])
   have cd2_suffix : cd2 <:+ cd.toChaseDerivationSkeleton := cd.branch.IsSuffix_drop n
   have node_head : node = cd2.head := by simp only [cd2, ChaseDerivationSkeleton.derivation_for_branch_suffix, ChaseDerivationSkeleton.head]; rcases Option.eq_some_iff_get_eq.mp node_eq with ⟨_, node_eq⟩; simp [← node_eq]
-  have cd2_branch : cd2.branch = cd.branch.drop n := rfl
-  have node2_mem : node2 ∈ (cd2.branch.drop m).head := by rw [cd2_branch]; grind
 
-  let cd3 : ChaseDerivationSkeleton obs rules := cd2.derivation_for_branch_suffix _ (cd2.branch.IsSuffix_drop m) (by rw [node2_mem]; simp)
-  have cd3_suffix : cd3 <:+ cd2 := cd2.branch.IsSuffix_drop m
-  have node2_head : node2 = cd3.head := by simp only [cd3, ChaseDerivationSkeleton.derivation_for_branch_suffix, ChaseDerivationSkeleton.head]; rw [Option.mem_def] at node2_mem; simp [node2_mem]
-
+  rcases (cd.derivation_for_skeleton cd2 cd2_suffix).growing' with ⟨cd3, suffix, t, t_not_mem, t_mem⟩
+  simp only [derivation_for_skeleton] at suffix
+  simp only [derivation_for_skeleton] at t_not_mem
   let node_cd2 : cd2.Node := ⟨node, by rw [node_head]; exact cd2.head_mem⟩
-  let node2_cd2 : cd2.Node := ⟨node2, by rw [node2_head]; apply cd3.mem_of_mem_suffix cd3_suffix; exact cd3.head_mem⟩
+  let node2_cd2 : cd2.Node := ⟨cd3.head, by apply cd3.mem_of_mem_suffix suffix; exact cd3.head_mem⟩
   have prec : node_cd2 ≺ node2_cd2 := by
     constructor
     . exists cd2; constructor; exact PossiblyInfiniteList.IsSuffix_refl; constructor; rw [← node_head]; exact node2_cd2.property
-    . intro contra; rw [Subtype.mk.injEq] at contra; apply t_not_mem; rw [contra]; exact t_mem
-
+    . intro contra; rw [Subtype.mk.injEq] at contra; apply t_not_mem; rw [← node_head, contra]; exact t_mem
   exists node2_cd2.cast_suffix cd2_suffix; constructor
   . show node_cd2.cast_suffix cd2_suffix ≺ node2_cd2.cast_suffix cd2_suffix
     apply ChaseDerivationSkeleton.strict_predecessor_of_suffix
     exact prec
-  . exists t
+  . exists t; simp only [node_head, t_not_mem, node2_cd2, not_false_iff, true_and]; exact t_mem
 
 /-- Since the derivation is growing, a next node always exists. -/
 theorem isSome_next {cd : CyclicityDerivation obs rules} : cd.toChaseDerivationSkeleton.next.isSome := by
-  rcases growing' ⟨cd.head, cd.head_mem⟩ with ⟨n2, prec, _⟩
+  rcases growing'' ⟨cd.head, cd.head_mem⟩ with ⟨n2, prec, _⟩
   have n2_mem := n2.property
   rw [ChaseDerivationSkeleton.mem_iff_eq_head_or_mem_tail] at n2_mem
   cases n2_mem with
@@ -173,7 +203,7 @@ theorem result_infinite {cd : CyclicityDerivation obs rules} : ¬ cd.result.fini
   have sub_res : l.toSet ⊆ cd.result := by intro e e_mem; rw [← eq, ← List.mem_toSet]; exact e_mem
   have res_sub : cd.result ⊆ l.toSet := by intro e e_mem; rw [List.mem_toSet, eq]; exact e_mem
   rcases cd.facts_mem_some_node_of_mem_result l sub_res with ⟨node, node_mem, sub⟩
-  rcases growing' ⟨node, node_mem⟩ with ⟨node2, prec, ⟨t, t_not_mem, t_mem⟩⟩
+  rcases growing'' ⟨node, node_mem⟩ with ⟨node2, prec, ⟨t, t_not_mem, t_mem⟩⟩
   apply t_not_mem
   apply FactSet.terms_subset_of_subset sub
   apply FactSet.terms_subset_of_subset res_sub
@@ -184,7 +214,7 @@ theorem result_infinite {cd : CyclicityDerivation obs rules} : ¬ cd.result.fini
 theorem infinite {cd : CyclicityDerivation obs rules} : ¬ cd.terminates := by
   intro contra
   rcases cd.has_last_node_of_terminates contra with ⟨node, node_last⟩
-  rcases cd.growing' node with ⟨node2, prec, ⟨t, t_not_mem, t_mem⟩⟩
+  rcases cd.growing'' node with ⟨node2, prec, ⟨t, t_not_mem, t_mem⟩⟩
   apply t_not_mem
   apply FactSet.terms_subset_of_subset (cd.facts_node_subset_of_prec (node_last node2))
   exact t_mem
@@ -192,26 +222,70 @@ theorem infinite {cd : CyclicityDerivation obs rules} : ¬ cd.terminates := by
 /-- In every `TreeDerivation` that starts on the same initial fact set as the `CyclicityDerivation`, there exists a branch that corresponds to the `CyclicityDerivation`, meaning that it has the same result. -/
 theorem corresponding_tree_branch_exists {cd : CyclicityDerivation obs rules} (td : TreeDerivation obs rules) (same_start : cd.head.facts = td.root.facts) :
     ∃ deriv ∈ td.branches, cd.result ⊆ deriv.result := by
-  let β := { pair : CyclicityDerivation obs rules × td.NodeWithAddress // pair.fst.head.facts ⊆ pair.snd.node.facts}
+  -- NOTE: The need for the suffix part of the property might not be obvious. This is required to show `different_value_exists` down below. For this we need to ensure that every possible value for β is already restricted to adhering to the suffix property. The more general claim without this property would not hold.
+  let β := { pair : CyclicityDerivation obs rules × td.NodeWithAddress // pair.fst.head.facts ⊆ pair.snd.node.facts ∧ pair.fst.toChaseDerivationSkeleton <:+ cd.toChaseDerivationSkeleton}
   let mapper : β -> td.NodeWithAddress := Prod.snd ∘ Subtype.val
-  let start : β := ⟨(cd, TreeDerivation.NodeWithAddress.root td), by rw [same_start]; simp only [TreeDerivation.NodeWithAddress.root]; exact Set.subset_refl⟩
+  let start : β := ⟨(cd, TreeDerivation.NodeWithAddress.root td), by
+    constructor
+    . rw [same_start]; simp only [TreeDerivation.NodeWithAddress.root]; exact Set.subset_refl
+    . exact PossiblyInfiniteList.IsSuffix_refl⟩
   let generator : β -> β := fun b =>
     let next := b.val.fst.next
     let origin := next.origin.get b.val.fst.isSome_origin_next
     have unblk := b.val.fst.unblockable next b.val.fst.next_mem origin (by simp [origin]) td b.val.snd (by
       have loaded : origin.fst.val.loaded b.val.fst.head.facts := b.val.fst.loaded_trigger_origin_next
       apply Set.subset_trans loaded
-      exact b.property)
+      exact b.property.left)
     let new_snd := Classical.choose unblk
     have new_snd_spec := Classical.choose_spec unblk
     ⟨(b.val.fst.tail, new_snd), by
-      simp only
-      rw [head_tail, b.val.fst.facts_next]
-      rw [Set.union_subset_iff_both_subset]; constructor
-      . apply Set.subset_trans b.property
-        exact td.facts_node_subset_of_prec new_snd_spec.left
-      . exact new_snd_spec.right⟩
-  have different_value_exists : ∀ b, ∃ n, mapper (generator.repeat_fun n b) ≠ mapper b := by sorry
+      constructor
+      . simp only
+        rw [head_tail, b.val.fst.facts_next]
+        rw [Set.union_subset_iff_both_subset]; constructor
+        . apply Set.subset_trans b.property.left
+          exact td.facts_node_subset_of_prec new_snd_spec.left
+        . exact new_snd_spec.right
+      . exact PossiblyInfiniteList.IsSuffix_trans PossiblyInfiniteList.IsSuffix_tail b.property.right⟩
+  have firstComponent_branch_eq : ∀ b, ∀ i, b.val.fst.branch.drop i = ((InfiniteList.iterate b generator).get i).val.fst.branch := by
+      intro b i
+      induction i with
+      | zero => rw [← InfiniteList.head_eq, InfiniteList.head_iterate]; simp
+      | succ i ih =>
+        rw [InfiniteList.get_iterate] at ih
+        rw [InfiniteList.get_succ_iterate]
+        conv => right; right; right; right; right; fun; unfold generator
+        simp only [tail, ChaseDerivationSkeleton.tail, derivation_for_skeleton, ChaseDerivationSkeleton.derivation_for_branch_suffix]
+        rw [← ih]
+        simp
+  have different_value_exists : ∀ b, ∃ n, mapper (generator.repeat_fun n b) ≠ mapper b := by
+    intro b
+    suffices ∀ l : List (GroundTerm sig), ∃ n, ∃ t,
+        t ∈ (td.generatedFacts (generator.repeat_fun n b).val.fst.head).terms ∧ t ∉ l by
+      rcases FactSet.terms_finite_of_finite _ (td.generatedFacts_finite_of_mem (mapper b).mem) with ⟨ts, _, ts_eq⟩
+      rcases this ts with ⟨n, t, t_mem, t_nmem⟩
+      exists n
+      intro contra
+      apply t_nmem
+      rw [ts_eq, ← contra]
+      rcases t_mem with ⟨f, f_mem, t_mem⟩
+      exists f; simp only [t_mem, and_true]
+      constructor
+      . exact (generator.repeat_fun n b).property.left _ f_mem.left
+      . exact f_mem.right
+    intro l
+    rcases b.val.fst.growing'_for_list l with ⟨cd2, suf, t, t_not_mem, t_mem, t_not_mem_l⟩
+    rw [ChaseDerivationSkeleton.IsSuffix_iff] at suf; rcases suf with ⟨n, suf⟩
+    exists n, t; simp only [t_not_mem_l, not_false_iff, and_true]
+    simp only [ChaseDerivationSkeleton.head, ← suf, firstComponent_branch_eq, InfiniteList.get_iterate] at t_mem
+    simp only [ChaseDerivationSkeleton.head]
+    rcases t_mem with ⟨f, f_mem, t_mem⟩
+    exists f; simp only [t_mem, and_true]; constructor; exact f_mem
+    rw [← same_start]
+    intro contra; apply t_not_mem
+    exists f; simp only [t_mem, and_true]
+    apply cd.facts_node_subset_every_mem _ _ _ contra
+    apply ChaseDerivationSkeleton.mem_of_mem_suffix b.property.right; exact b.val.fst.head_mem
   let condensed_generator := Function.condense_generator generator mapper different_value_exists
   let deriv := td.generate_subderivation_from_sparse_of_total_generator start condensed_generator mapper (by
     suffices ∀ b n, mapper b ≼ mapper (generator.repeat_fun n b) by
@@ -231,7 +305,7 @@ theorem corresponding_tree_branch_exists {cd : CyclicityDerivation obs rules} (t
       have unblk := (generator.repeat_fun n b).val.fst.unblockable next (generator.repeat_fun n b).val.fst.next_mem origin (by simp [origin]) td (generator.repeat_fun n b).val.snd (by
         have loaded : origin.fst.val.loaded (generator.repeat_fun n b).val.fst.head.facts := (generator.repeat_fun n b).val.fst.loaded_trigger_origin_next
         apply Set.subset_trans loaded
-        exact (generator.repeat_fun n b).property)
+        exact (generator.repeat_fun n b).property.left)
       exact (Classical.choose_spec unblk).left)
 
   exists deriv; constructor
@@ -246,7 +320,7 @@ theorem corresponding_tree_branch_exists {cd : CyclicityDerivation obs rules} (t
       . rw [← deriv.mem_def]
         apply td.mem_generate_subderivation_from_sparse_of_total_generator_of_mem_original_generator
         exact b_mem
-      . apply b.property
+      . apply b.property.left
         rw [node2_mem]
         apply ChaseDerivationSkeleton.facts_node_subset_of_prec prec
         exact f_mem
@@ -268,19 +342,7 @@ theorem corresponding_tree_branch_exists {cd : CyclicityDerivation obs rules} (t
           exists j
           rw [InfiniteList.get_iterate]
         . rfl
-    suffices ∀ i, ∃ j, (condensed_generator.repeat_fun j start).val.fst.toChaseDerivationSkeleton <:+ (generator.repeat_fun i start).val.fst.toChaseDerivationSkeleton by
-      suffices branch_eq : ∀ i, cd.branch.drop i = ((InfiniteList.iterate start generator).get i).val.fst.branch by
-        intro i; rw [branch_eq i]; simp only [InfiniteList.get_iterate]; exact this i
-      intro i
-      induction i with
-      | zero => rw [← InfiniteList.head_eq, InfiniteList.head_iterate]; simp [start]
-      | succ i ih =>
-        rw [InfiniteList.get_iterate] at ih
-        rw [InfiniteList.get_succ_iterate]
-        conv => right; right; right; right; right; fun; unfold generator
-        simp only [tail, ChaseDerivationSkeleton.tail, derivation_for_skeleton, ChaseDerivationSkeleton.derivation_for_branch_suffix]
-        rw [← ih]
-        simp
+    suffices ∀ i, ∃ j, (condensed_generator.repeat_fun j start).val.fst.toChaseDerivationSkeleton <:+ (generator.repeat_fun i start).val.fst.toChaseDerivationSkeleton by intro i; rw [firstComponent_branch_eq start i]; simp only [InfiniteList.get_iterate]; exact this i
     suffices ∀ b i, (generator.repeat_fun i b).val.fst.toChaseDerivationSkeleton <:+ b.val.fst.toChaseDerivationSkeleton by
       suffices condensed_exceeds_generator : ∀ b i, ∃ j k, (condensed_generator.repeat_fun j b) = (generator.repeat_fun (i+k) b) by
         intro i; rcases condensed_exceeds_generator start i with ⟨j, k, eq⟩
